theories/heap_lang/notation.v
@@ -10,6 +10,7 @@ Coercion LitInt : Z >-> base_lit.
 Coercion LitBool : bool >-> base_lit.
 Coercion LitLoc : loc >-> base_lit.
 Coercion LitProphecy : proph_id >-> base_lit.
+Coercion LitTag : string >-> base_lit.
 
 Coercion App : expr >-> Funclass.
 
